\chapter{Important Formulas} % Chapter 1

This is a test of the section. JWK

\section{Linear Functions}
\subsection{Slope-Intercept Form}
\begin{equation} 
    f(x) = mx + b
\end{equation}

\subsection{Point-Slope Form}
\begin{equation}
    y-y_1 = m(x - x_1)
\end{equation}
\subsection{Standard Form}
\begin{equation}
    ax+by = c,
\end{equation}
\begin{equation}
    a+b \neq 0 
\end{equation}
\subsection{Slope Formula}
\begin{equation}
    m = \frac{y_2 - y_1}{x_2 - x_1}
\end{equation}

\section{Quadratic Functions}
\subsection{Vertex Form}
\begin{equation}
    f(x) = a(x-h)^2 + k
\end{equation}

\subsection{Standard Form}
\begin{equation}
    f(x) = ax^2 + bx + c
\end{equation}

\subsection{Quadratic Formula}
\begin{equation}
	x = \frac{-b \pm \sqrt{b^2 - 4ac}}{2a}
\end{equation}

\section{Exponential Functions}
\subsection{Exponential Growth}
\begin{equation}
    f(x) = ab^x
\end{equation}

\subsection{Exponential Decay}
\begin{equation}
    f(x) = ab^{-x}
\end{equation}

\section{Logarithmic Functions}
\subsection{Common Logarithm}
\begin{equation}
    f(x) = \log_b(x)
\end{equation}

\subsection{Natural Logarithm}
\begin{equation}
    f(x) = \ln(x)
\end{equation}

\section{Trigonometric Functions}
\subsection{Sine Function}
\begin{equation}
    f(x) = \sin(x)
\end{equation}

\subsection{Cosine Function}
\begin{equation}
    f(x) = \cos(x)
\end{equation}

\subsection{Tangent Function}
\begin{equation}
    f(x) = \tan(x)
\end{equation}

\section{Limits}
\subsection{Definition of a Limit}
\begin{equation}
    \lim_{x \to a} f(x) = L
\end{equation}

\subsection{Limit Laws}
\begin{equation}
    \lim_{x \to a} [f(x) + g(x)] = \lim_{x \to a} f(x) + \lim_{x \to a} g(x)
\end{equation}

\begin{equation}
    \lim_{x \to a} [f(x) - g(x)] = \lim_{x \to a} f(x) - \lim_{x \to a} g(x)
\end{equation}

\begin{equation}
    \lim_{x \to a} [cf(x)] = c \lim_{x \to a} f(x)
\end{equation}

\begin{equation}
    \lim_{x \to a} [f(x)g(x)] = \lim_{x \to a} f(x) \lim_{x \to a} g(x)
\end{equation}

\begin{equation}
    \lim_{x \to a} \frac{f(x)}{g(x)} = \frac{\lim_{x \to a} f(x)}{\lim_{x \to a} g(x)}
\end{equation}

\begin{equation}
    \lim_{x \to a} [f(x)]^n = [\lim_{x \to a} f(x)]^n
\end{equation}

\begin{equation}
    \lim_{x \to a} \sqrt[n]{f(x)} = \sqrt[n]{\lim_{x \to a} f(x)}
\end{equation}

\begin{equation}
    \lim_{x \to a} \sqrt[n]{f(x)} = \sqrt[n]{\lim_{x \to a} f(x)}
\end{equation}

\begin{equation}
    \lim_{x \to a} f(x)^{g(x)} = \left[\lim_{x \to a} f(x)\right]^{\lim_{x \to a} g(x)}
\end{equation}

\begin{equation}
    \lim_{x \to a} \frac{1}{f(x)} = \frac{1}{\lim_{x \to a} f(x)}
\end{equation}

\begin{equation}
    \lim_{x \to a} \frac{1}{f(x)} = \frac{1}{\lim_{x \to a} f(x)}
\end{equation}

\begin{equation}
    \lim_{x \to a} \frac{1}{f(x)} = \frac{1}{\lim_{x \to a} f(x)}
\end{equation}

\begin{equation}
    \lim_{x \to a} \frac{1}{f(x)} = \frac{1}{\lim_{x \to a} f(x)}
\end{equation}

\begin{equation}
    \lim_{x \to a} \frac{1}{f(x)} = \frac{1}{\lim_{x \to a} f(x)}
\end{equation}